InsertLeaf

examples/MutableBtree.dfy
@@ -48,6 +48,7 @@ abstract module MutableBtree {
     if node.NotInUse? then false
     else if node.Leaf? then
       && node.repr == { node.keys, node.values }
+      && node.keys != node.values
       && 0 <= node.nkeys as int <= MaxKeysPerLeaf() as int == node.keys.Length
       && node.values.Length == node.keys.Length
     else 
@@ -205,6 +206,8 @@ abstract module MutableBtree {
   function I(node: Node) : (result: BS.Node)
     requires WFShape(node)
     ensures node.Leaf? ==> result.Leaf?
+    ensures node.Leaf? ==> result.keys == node.keys[..node.nkeys];
+    ensures node.Leaf? ==> result.values == node.values[..node.nkeys];
     ensures node.Index? ==> result.Index?
     ensures node.Index? ==> result.pivots == node.pivots[..node.nchildren-1]
     ensures node.Index? ==> |result.children| == node.nchildren as int
@@ -281,24 +284,32 @@ abstract module MutableBtree {
   {
     BS.SplitLeaf(oldleaf, leftleaf, rightleaf, pivot)
   }
-    
+
   predicate {:opaque} BSSplitIndex(oldleaf: BS.Node, leftleaf: BS.Node, rightleaf: BS.Node, pivot: Key)
   {
     BS.SplitIndex(oldleaf, leftleaf, rightleaf, pivot)
   }
-    
+
   predicate {:opaque} BSSplitNode(oldleaf: BS.Node, leftleaf: BS.Node, rightleaf: BS.Node, pivot: Key)
   {
     BS.SplitNode(oldleaf, leftleaf, rightleaf, pivot)
   }
-    
+
   predicate {:opaque} BSSplitChildOfIndex(oldindex: BS.Node, newindex: BS.Node, childidx: int)
     requires oldindex.Index?
     requires 0 <= childidx < |oldindex.children|
   {
     BS.SplitChildOfIndex(oldindex, newindex, childidx)
   }
-    
+
+  function {:opaque} BSInsertLeaf(leaf: BS.Node, key: Key, value: Value) : (result: BS.Node)
+    requires leaf.Leaf?
+    requires BSWF(leaf)
+  {
+    reveal_BSWF();
+    BS.InsertLeaf(leaf, key, value)
+  }
+  
   lemma IndexPrefixIsSubIndex(node: Node, newnchildren: int)
     requires WFShape(node)
     requires BSWF(I(node))
@@ -635,191 +646,32 @@ abstract module MutableBtree {
     }
     SplitChildOfIndexIsBSSplitChildOfIndex(old(I(node)), I(newnode), childidx as int);
   }
-   
-  //   // method Insert(key: Key, value: Value)
-  //   //   requires WF()
-  //   //   requires !Full()
-  //   //   ensures WF()
-  //   //   ensures Interpretation() == old(Interpretation())[key := value]
-  //   //   ensures AllKeys() == old(AllKeys()) + {key}
-  //   //   ensures fresh(subtreeObjects-old(subtreeObjects))
-  //   //   modifies this, subtreeObjects
-  //   //   decreases AllKeys()
-  //   // {
-  //   //   var posplus1 := Keys.ArrayLargestLtePlus1(keys, 0, nkeys, key);
 
-  //   //   if 1 <= posplus1 && keys[posplus1-1] == key {
-  //   //     values[posplus1-1] := value;
-  //   //   } else {
-  //   //     ghost var oldkeys := keys[..nkeys];
-  //   //     Arrays.Insert(keys, nkeys, key, posplus1);
-  //   //     Arrays.Insert(values, nkeys, value, posplus1);
-  //   //     nkeys := nkeys + 1;
+  method InsertLeaf(node: Node, key: Key, value: Value) returns (result: Node)
+    requires WFShape(node)
+    requires BSWF(I(node))
+    requires node.Leaf?
+    requires !Full(node)
+    ensures WFShape(result)
+    ensures result.repr == node.repr
+    ensures result.Leaf?
+    ensures I(result) == BSInsertLeaf(old(I(node)), key, value)
+    modifies node.keys, node.values
+  {
+    reveal_BSWF();
+    reveal_BSInsertLeaf();
 
-  //   //     InsertMultiset(oldkeys, key, posplus1 as int); // OBSERVE
-  //   //     Keys.strictlySortedInsert(oldkeys, key, posplus1 as int - 1); // OBSERVE
-  //   //     Keys.PosEqLargestLte(keys[..nkeys], key, posplus1 as int);
-  //   //     forall key' |  key' != key && key' in old(Interpretation())
-  //   //       ensures key' in Interpretation() && Interpretation()[key'] == old(Interpretation())[key']
-  //   //     {
-  //   //       var i: int := Keys.LargestLte(old(keys[..nkeys]), key');
-  //   //       //assert 0 <= i;
-  //   //       if i < posplus1 as int {
-  //   //         //assert keys[i] == key';
-  //   //         Keys.PosEqLargestLte(keys[..nkeys], key', i);
-  //   //       } else {
-  //   //         //assert keys[i+1] == key';
-  //   //         Keys.PosEqLargestLte(keys[..nkeys], key', i+1);
-  //   //       }
-  //   //     }
-  //   //     forall key' | key' != key && key' in Interpretation()
-  //   //       ensures key' in old(Interpretation()) && old(Interpretation())[key'] == Interpretation()[key']
-  //   //     {
-  //   //       var i: int := Keys.LargestLte(keys[..nkeys], key');
-  //   //       if i < posplus1 as int {
-  //   //         Keys.PosEqLargestLte(old(keys[..nkeys]), key', i);
-  //   //       } else {
-  //   //         Keys.PosEqLargestLte(old(keys[..nkeys]), key', i-1);
-  //   //       }
-  //   //     }
-  //   //   }
-  //   // }
-
-  //   // constructor()
-  //   //   ensures WF()
-  //   //   ensures Interpretation() == map[]
-  //   //   ensures !Full()
-  //   //   ensures fresh(keys)
-  //   //   ensures fresh(values)
-  //   // {
-  //   //   nkeys := 0;
-  //   //   keys := new Key[MaxKeysPerLeaf()](_ => DefaultKey());
-  //   //   values := new Value[MaxKeysPerLeaf()](_ => DefaultValue());
-  //   //   subtreeObjects := {this, keys, values};
-  //   // }
-  // }
-
-  // class Index extends Node {
-  //   var nchildren: uint64
-  //   var pivots: array<Key>
-  //   var children: array<NodeBox>
-
-
-  //   // lemma AllKeysStrictlyDecreasing()
-  //   //   requires WF()
-  //   //   ensures forall i :: 0 <= i < nchildren ==> children[i].node.allKeys < allKeys
-  //   // {
-  //   //   forall i | 0 <= i < nchildren
-  //   //     ensures children[i].node.allKeys < allKeys
-  //   //   {
-  //   //     var i' := if i < nchildren-1 then i+1 else 0;
-  //   //     assert i' != i;
-  //   //     assert children[i].node.allKeys !! children[i'].node.allKeys;
-  //   //     assert children[i].node.allKeys <= 
-  //   //     assert children[i].node.allKeys <= allKeys;
-  //   //   }
-  //   // }
-    
-  //   // method SplitChild(key: Key, childidx: uint64)
-  //   //   requires WF()
-  //   //   requires !Full()
-  //   //   requires childidx as int == 1 + Keys.LargestLte(pivots[..nchildren-1], key)
-  //   //   requires children[childidx].node.Full()
-  //   //   ensures WF()
-  //   //   //ensures Interpretation() == old(Interpretation())
-  //   //   ensures SplitChildOfIndex(old(ToImmutableNode()), ToImmutableNode(), childidx as int)
-  //   //   ensures fresh(subtreeObjects-old(subtreeObjects))
-  //   //   modifies this, pivots, children, children[childidx].node
-  //   // {
-  //   //   ghost var oldchildren := children;
-      
-  //   //   var pivot, right := children[childidx].node.Split();
-  //   //   Arrays.Insert(pivots, nchildren - 1, pivot, childidx);
-  //   //   Arrays.Insert(children, nchildren, NodeBox(right), childidx + 1);
-  //   //   nchildren := nchildren + 1;
-  //   //   subtreeObjects := subtreeObjects + right.subtreeObjects;
-
-      
-  //   //   // Keys.LargestLteIsUnique(old(pivots[..nchildren-1]), pivot, childidx as int - 1);
-  //   //   // Keys.strictlySortedInsert(old(pivots[..nchildren-1]), pivot, childidx as int - 1);
-
-  //   //   assert forall i: uint64 :: 0 <= i < childidx ==> children[i] == oldchildren[i];
-  //   //   assert children[childidx as int + 1].node == right;
-  //   //   assert forall i: uint64 :: childidx + 1 < i < nchildren ==> children[i] == oldchildren[i-1];
-  //   //   // forall i: int, j: int {:trigger children[i].node.subtreeObjects, children[j].node.subtreeObjects}
-  //   //   // | 0 <= i < j < nchildren as int
-  //   //   //   ensures children[i].node.subtreeObjects !! children[j].node.subtreeObjects
-  //   //   // {
-  //   //   //   if                                   j  < childidx as int {
-  //   //   //   } else if                            j == childidx as int {
-  //   //   //   } else if i  < childidx as int     && j == childidx as int + 1 {
-  //   //   //   } else if i == childidx as int     && j == childidx as int + 1 {
-  //   //   //   } else if i  < childidx as int     && j  > childidx as int + 1 {
-  //   //   //   } else if i == childidx as int     && j  > childidx as int + 1 {
-  //   //   //   } else if i == childidx as int + 1 && j  > childidx as int + 1 {
-  //   //   //   } else {
-  //   //   //   }
-  //   //   // }
-  //   //   // // forall i: int, key | 0 <= i < (nchildren as int)-1 && key in children[i].node.allKeys
-  //   //   // //   ensures Keys.lt(key, pivots[i])
-  //   //   // // {
-  //   //   // //   if childidx as int + 1 < i {
-  //   //   // //     assert children[i] == old(children[i-1]);
-  //   //   // //   }
-  //   //   // // }
-  //   //   // // forall i: int, key | 0 < i < nchildren as int && key in children[i].node.allKeys
-  //   //   // //   ensures Keys.lt(pivots[i-1], key)
-  //   //   // // {
-  //   //   // //   if i < childidx as int {
-  //   //   // //     assert Keys.lt(pivots[i-1], key);
-  //   //   // //   } else if i == childidx as int {
-  //   //   // //     assert Keys.lt(pivots[i-1], key);
-  //   //   // //   } else if i == childidx as int + 1 {
-  //   //   // //     assert Keys.lt(pivots[i-1], key);
-  //   //   // //   } else {
-  //   //   // //     assert Keys.lt(pivots[i-1], key);
-  //   //   // //   }
-  //   //   // // }
-  //   //   // assert WF();
-        
-  //   //   // forall key | key in old(Interpretation())
-  //   //   //   ensures key in Interpretation() && Interpretation()[key] == old(Interpretation()[key])
-  //   //   // {
-  //   //   //   var llte: int := Keys.LargestLte(old(pivots[..nchildren-1]), key);
-  //   //   //   assert key in old(children[llte+1].node.Interpretation());
-  //   //   //   assert old(children[llte+1].node.Interpretation()[key]) == old(Interpretation()[key]);
-  //   //   //   if llte < childidx as int {
-  //   //   //     assert key in Interpretation() && Interpretation()[key] == old(Interpretation()[key]);
-  //   //   //   } else if llte == childidx as int {
-  //   //   //     if Keys.lt(key, pivot) {
-  //   //   //       assert key in Interpretation() && Interpretation()[key] == old(Interpretation()[key]);
-  //   //   //     } else {
-  //   //   //       assert key in Interpretation() && Interpretation()[key] == old(Interpretation()[key]);
-  //   //   //     }
-  //   //   //   } else {
-  //   //   //     assert key in Interpretation() && Interpretation()[key] == old(Interpretation()[key]);
-  //   //   //   }
-  //   //   // }
-  //   //   // forall key | key in Interpretation()
-  //   //   //   ensures key in old(Interpretation()) && Interpretation()[key] == old(Interpretation()[key])
-  //   //   // {
-  //   //   //   var llte: int := Keys.LargestLte(pivots[..nchildren-1], key);
-  //   //   //   if llte < childidx as int {
-  //   //   //   } else if llte == childidx as int {
-  //   //   //   } else if llte == childidx as int + 1 {
-  //   //   //   } else {
-  //   //   //   }
-  //   //   // }
-  //   // }
-    
-  //   // function UnionSubtreeObjects() : set<object>
-  //   //   requires nchildren as int <= children.Length
-  //   //   requires forall i :: 0 <= i < nchildren ==> children[i].node != null
-  //   //   reads this, children, set i | 0 <= i < nchildren :: children[i].node
-  //   // {
-  //   //   set o, i | 0 <= i < nchildren && o in children[i].node.subtreeObjects :: o
-  //   // }
-    
+    var posplus1: uint64 := BS.Keys.ArrayLargestLtePlus1(node.keys, 0, node.nkeys, key);
+    if 1 <= posplus1 && node.keys[posplus1-1] == key {
+      node.values[posplus1-1] := value;
+      result := node;
+    } else {
+      Arrays.Insert(node.keys, node.nkeys, key, posplus1);
+      Arrays.Insert(node.values, node.nkeys, value, posplus1);
+      result := node.(nkeys := node.nkeys + 1);
+    }
+  }
+  
   //   // // method Insert(key: Key, value: Value)
   //   // //   requires WF()
   //   // //   requires !Full()
